vale/code/arch/x64/Vale.X64.Memory.fsti
@@ -4,21 +4,38 @@ open FStar.Mul
 open Vale.Def.Prop_s
 open Vale.X64.Machine_s
 open Vale.Arch.HeapImpl
+module Map16 = Vale.Lib.Map16
 
 unfold let vale_heap = vale_heap
 unfold let vale_full_heap = vale_full_heap
+unfold let heaplet_id = heaplet_id
 
 [@"opaque_to_smt"]
-let get_vale_heap (vhi:vale_full_heap) : vale_heap = vhi.v_h
-let get_one_vale_heap (vhi:vale_full_heap) : vale_heap = vhi.v_h
-let set_vale_heap (vhi:vale_full_heap) (vh:vale_heap) : vale_full_heap = {v_h = vh}
+let get_vale_heap (vhi:vale_full_heap) : vale_heap = vhi.vf_heap
+
+let get_one_vale_heap (vhi:vale_full_heap) : vale_heap = vhi.vf_heap
+
+let set_vale_heap (vfh:vale_full_heap) (vh:vale_heap) : vale_full_heap =
+  {vf_layout = vfh.vf_layout; vf_heap = vh; vf_heaplets = vfh.vf_heaplets}
+
 let lemma_set_vale_heap (vhi:vale_full_heap) (vh:vale_heap) : Lemma
   (requires True)
   (ensures get_vale_heap (set_vale_heap vhi vh) == vh)
   [SMTPat (set_vale_heap vhi vh)]
   =
   FStar.Pervasives.reveal_opaque (`%get_vale_heap) get_vale_heap
-let vale_full_heap_equal (h1 h2:vale_full_heap) = get_one_vale_heap h1 == get_one_vale_heap h2
+
+let vale_full_heap_equal (h1 h2:vale_full_heap) =
+  get_one_vale_heap h1 == get_one_vale_heap h2 /\
+  h1.vf_layout == h2.vf_layout /\
+  Map16.equal h1.vf_heaplets h2.vf_heaplets
+
+let lemma_vale_full_heap_equal (h1 h2:vale_full_heap) : Lemma
+  (requires vale_full_heap_equal h1 h2)
+  (ensures h1 == h2)
+  [SMTPat (vale_full_heap_equal h1 h2)]
+  =
+  FStar.Pervasives.reveal_opaque (`%get_vale_heap) get_vale_heap
 
 unfold let nat8 = Vale.Def.Words_s.nat8
 unfold let nat16 = Vale.Def.Words_s.nat16
