vale/code/arch/Vale.Arch.Heap.fst
@@ -6,9 +6,13 @@ friend Vale.Arch.HeapImpl
 
 let heap_impl = vale_full_heap
 
-let heap_get hi = hi.v_h.mh
+let heap_get hi = hi.vf_heap.mh
 
 let heap_upd hi mh' =
-  {v_h = mi_heap_upd hi.v_h mh'}
+  {vf_layout = hi.vf_layout; vf_heap = mi_heap_upd hi.vf_heap mh'; vf_heaplets = hi.vf_heaplets}
 
-let heap_create_from_interop ih = {v_h = ValeHeap (down_mem ih) (Ghost.hide ih)}
+let heap_create_from_interop ih =
+  let vh = ValeHeap (down_mem ih) (Ghost.hide ih) in
+  let vh4 = ((vh, vh), (vh, vh)) in
+  let vh16 = ((vh4, vh4), (vh4, vh4)) in
+  {vf_layout = {vl_old_heap = vh}; vf_heap = vh; vf_heaplets = vh16}
